\documentclass{article}

\usepackage{amsmath}

\begin{document}

\begin{equation}\tag{2}\label{eq2}\begin{aligned}
a &= b + c \\
  &= d + e + f + g \\
  &= h + i
\end{aligned}\end{equation}

\begin{equation}\begin{aligned}
a &= b + c \\
  &= d + e + f + g \\
  &= h + i
\end{aligned}\tag{2}\label{eq2}\end{equation}

\begin{align}
\sqrt{37} &= \sqrt{\frac{73^2-1}{12^2}} \\
 &= \sqrt{\frac{73^2}{12^2}\cdot\frac{73^2-1}{73^2}} \\
 &= \sqrt{\frac{73^2}{12^2}}\sqrt{\frac{73^2-1}{73^2}} \\
 &= \frac{73}{12}\sqrt{1 - \frac{1}{73^2}} \\
 &\approx \frac{73}{12}\left(1 - \frac{1}{2\cdot73^2}\right)
\end{align}

\end{document}


\begin{equation}\tag{2}\label{eq2}\begin{aligned}a &= b + c \\  &= d + e + f + g \\  &= h + i\end{aligned}\end{equation}

\\begin{align}\\sqrt{37} &= \\sqrt{\\frac{73^2-1}{12^2}} \\\\ &= \\sqrt{\\frac{73^2}{12^2}\\cdot\\frac{73^2-1}{73^2}} \\\\ &= \\sqrt{\\frac{73^2}{12^2}}\\sqrt{\\frac{73^2-1}{73^2}} \\\\ &= \\frac{73}{12}\\sqrt{1 - \\frac{1}{73^2}} \\\\ &\\approx \\frac{73}{12}\\left(1 - \\frac{1}{2\\cdot73^2}\\right)\\end{align}
