\documentclass{article}
\usepackage{empheq}
\usepackage{cases}

\begin{document}
  \begin{numcases}{\theta _{ij}(\rho )=} \tag{2.9} \theta _{ij}^{U}(\rho )=\rho _{i}, \; \text{if}\; S_{j}>S_{i},&\\\tag{2.10} \theta _{ij}^{A}(\rho )=\frac{\rho _{i}+\rho _{j}}{2} &\\\tag{2.11} \theta _{ij}^{L}(\rho )=\frac{\rho _{i}-\rho _{j}}{\log (\rho _{i})-\log (\rho _{j})}. &\\\end{numcases}


  \begin{numcases}{\theta _{ij}(\rho )=} \theta _{ij}^{U}(\rho )=\rho _{i}, \; \text{if}\; S_{j}>S_{i},&\\ \theta _{ij}^{A}(\rho )=\frac{\rho _{i}+\rho _{j}}{2} &\\ \theta _{ij}^{L}(\rho )=\frac{\rho _{i}-\rho _{j}}{\log (\rho _{i})-\log (\rho _{j})}. &\\\end{numcases}

  \begin{subnumcases}{\theta _{ij}(\rho )=} \theta _{ij}^{U}(\rho )=\rho _{i}, \; \text{if}\; S_{j}>S_{i},&\\ \theta _{ij}^{A}(\rho )=\frac{\rho _{i}+\rho _{j}}{2} &\\ \theta _{ij}^{L}(\rho )=\frac{\rho _{i}-\rho _{j}}{\log (\rho _{i})-\log (\rho _{j})}. &\\\end{subnumcases}

\end{document}



